Implemented basic dynamic logic syntax + semantics. Changed file structure.

.lake/build/ir/Main.c
@@ -1,6 +1,6 @@
 // Lean compiler output
 // Module: Main
-// Imports: public import Init public import LeanExamples
+// Imports: public import Init public import Logic.Prop.Syntax public import Logic.Prop.Semantics public import Logic.DL.Syntax public import Logic.DL.Semantics
 #include <lean/lean.h>
 #if defined(__clang__)
 #pragma clang diagnostic ignored "-Wunused-parameter"
@@ -13,80 +13,128 @@
 #ifdef __cplusplus
 extern "C" {
 #endif
+lean_object* lp_lean__examples_Logic_DL_conj(lean_object*, lean_object*);
+uint8_t lean_string_dec_eq(lean_object*, lean_object*);
 LEAN_EXPORT lean_object* _lean_main();
 LEAN_EXPORT lean_object* lp_lean__examples_main___boxed(lean_object*);
-LEAN_EXPORT lean_object* lp_lean__examples_IO_print___at___00IO_println___at___00main_spec__0_spec__0___boxed(lean_object*, lean_object*);
-lean_object* lean_string_push(lean_object*, uint32_t);
-lean_object* lean_get_stdout();
-LEAN_EXPORT lean_object* lp_lean__examples_IO_println___at___00main_spec__0(lean_object*);
-static lean_object* lp_lean__examples_main___closed__0;
-LEAN_EXPORT lean_object* lp_lean__examples_IO_print___at___00IO_println___at___00main_spec__0_spec__0(lean_object*);
-LEAN_EXPORT lean_object* lp_lean__examples_IO_println___at___00main_spec__0___boxed(lean_object*, lean_object*);
-LEAN_EXPORT lean_object* lp_lean__examples_IO_print___at___00IO_println___at___00main_spec__0_spec__0(lean_object* x_1) {
+static const lean_string_object lp_lean__examples_f___closed__0_value = {.m_header = {.m_rc = 0, .m_cs_sz = 0, .m_other = 0, .m_tag = 249}, .m_size = 2, .m_capacity = 2, .m_length = 1, .m_data = "p"};
+static const lean_object* lp_lean__examples_f___closed__0 = (const lean_object*)&lp_lean__examples_f___closed__0_value;
+static const lean_ctor_object lp_lean__examples_f___closed__1_value = {.m_header = {.m_rc = 0, .m_cs_sz = sizeof(lean_ctor_object) + sizeof(void*)*1 + 0, .m_other = 1, .m_tag = 0}, .m_objs = {((lean_object*)&lp_lean__examples_f___closed__0_value)}};
+static const lean_object* lp_lean__examples_f___closed__1 = (const lean_object*)&lp_lean__examples_f___closed__1_value;
+static const lean_string_object lp_lean__examples_f___closed__2_value = {.m_header = {.m_rc = 0, .m_cs_sz = 0, .m_other = 0, .m_tag = 249}, .m_size = 2, .m_capacity = 2, .m_length = 1, .m_data = "q"};
+static const lean_object* lp_lean__examples_f___closed__2 = (const lean_object*)&lp_lean__examples_f___closed__2_value;
+static const lean_ctor_object lp_lean__examples_f___closed__3_value = {.m_header = {.m_rc = 0, .m_cs_sz = sizeof(lean_ctor_object) + sizeof(void*)*1 + 0, .m_other = 1, .m_tag = 0}, .m_objs = {((lean_object*)&lp_lean__examples_f___closed__2_value)}};
+static const lean_object* lp_lean__examples_f___closed__3 = (const lean_object*)&lp_lean__examples_f___closed__3_value;
+static const lean_ctor_object lp_lean__examples_f___closed__4_value = {.m_header = {.m_rc = 0, .m_cs_sz = sizeof(lean_ctor_object) + sizeof(void*)*2 + 0, .m_other = 2, .m_tag = 3}, .m_objs = {((lean_object*)&lp_lean__examples_f___closed__1_value),((lean_object*)&lp_lean__examples_f___closed__3_value)}};
+static const lean_object* lp_lean__examples_f___closed__4 = (const lean_object*)&lp_lean__examples_f___closed__4_value;
+LEAN_EXPORT const lean_object* lp_lean__examples_f = (const lean_object*)&lp_lean__examples_f___closed__4_value;
+LEAN_EXPORT uint8_t lp_lean__examples_I(lean_object*);
+LEAN_EXPORT lean_object* lp_lean__examples_I___boxed(lean_object*);
+LEAN_EXPORT lean_object* lp_lean__examples_model;
+static const lean_ctor_object lp_lean__examples_p___closed__0_value = {.m_header = {.m_rc = 0, .m_cs_sz = sizeof(lean_ctor_object) + sizeof(void*)*1 + 0, .m_other = 1, .m_tag = 0}, .m_objs = {((lean_object*)&lp_lean__examples_f___closed__0_value)}};
+static const lean_object* lp_lean__examples_p___closed__0 = (const lean_object*)&lp_lean__examples_p___closed__0_value;
+LEAN_EXPORT const lean_object* lp_lean__examples_p = (const lean_object*)&lp_lean__examples_p___closed__0_value;
+static const lean_ctor_object lp_lean__examples_q___closed__0_value = {.m_header = {.m_rc = 0, .m_cs_sz = sizeof(lean_ctor_object) + sizeof(void*)*1 + 0, .m_other = 1, .m_tag = 0}, .m_objs = {((lean_object*)&lp_lean__examples_f___closed__2_value)}};
+static const lean_object* lp_lean__examples_q___closed__0 = (const lean_object*)&lp_lean__examples_q___closed__0_value;
+LEAN_EXPORT const lean_object* lp_lean__examples_q = (const lean_object*)&lp_lean__examples_q___closed__0_value;
+static const lean_ctor_object lp_lean__examples_00_u03c6___closed__0_value = {.m_header = {.m_rc = 0, .m_cs_sz = sizeof(lean_ctor_object) + sizeof(void*)*1 + 0, .m_other = 1, .m_tag = 0}, .m_objs = {((lean_object*)(((size_t)(0) << 1) | 1))}};
+static const lean_object* lp_lean__examples_00_u03c6___closed__0 = (const lean_object*)&lp_lean__examples_00_u03c6___closed__0_value;
+static const lean_ctor_object lp_lean__examples_00_u03c6___closed__1_value = {.m_header = {.m_rc = 0, .m_cs_sz = sizeof(lean_ctor_object) + sizeof(void*)*2 + 0, .m_other = 2, .m_tag = 3}, .m_objs = {((lean_object*)&lp_lean__examples_00_u03c6___closed__0_value),((lean_object*)&lp_lean__examples_q___closed__0_value)}};
+static const lean_object* lp_lean__examples_00_u03c6___closed__1 = (const lean_object*)&lp_lean__examples_00_u03c6___closed__1_value;
+LEAN_EXPORT const lean_object* lp_lean__examples_00_u03c6 = (const lean_object*)&lp_lean__examples_00_u03c6___closed__1_value;
+static const lean_ctor_object lp_lean__examples_00_u03b1___closed__0_value = {.m_header = {.m_rc = 0, .m_cs_sz = sizeof(lean_ctor_object) + sizeof(void*)*1 + 0, .m_other = 1, .m_tag = 0}, .m_objs = {((lean_object*)(((size_t)(1) << 1) | 1))}};
+static const lean_object* lp_lean__examples_00_u03b1___closed__0 = (const lean_object*)&lp_lean__examples_00_u03b1___closed__0_value;
+static const lean_ctor_object lp_lean__examples_00_u03b1___closed__1_value = {.m_header = {.m_rc = 0, .m_cs_sz = sizeof(lean_ctor_object) + sizeof(void*)*2 + 0, .m_other = 2, .m_tag = 2}, .m_objs = {((lean_object*)&lp_lean__examples_00_u03b1___closed__0_value),((lean_object*)&lp_lean__examples_00_u03c6___closed__0_value)}};
+static const lean_object* lp_lean__examples_00_u03b1___closed__1 = (const lean_object*)&lp_lean__examples_00_u03b1___closed__1_value;
+LEAN_EXPORT const lean_object* lp_lean__examples_00_u03b1 = (const lean_object*)&lp_lean__examples_00_u03b1___closed__1_value;
+static const lean_ctor_object lp_lean__examples_00_u03b2___closed__0_value = {.m_header = {.m_rc = 0, .m_cs_sz = sizeof(lean_ctor_object) + sizeof(void*)*2 + 0, .m_other = 2, .m_tag = 3}, .m_objs = {((lean_object*)&lp_lean__examples_00_u03c6___closed__0_value),((lean_object*)&lp_lean__examples_00_u03b1___closed__0_value)}};
+static const lean_object* lp_lean__examples_00_u03b2___closed__0 = (const lean_object*)&lp_lean__examples_00_u03b2___closed__0_value;
+LEAN_EXPORT const lean_object* lp_lean__examples_00_u03b2 = (const lean_object*)&lp_lean__examples_00_u03b2___closed__0_value;
+static const lean_ctor_object lp_lean__examples_00_u03c8___closed__0_value = {.m_header = {.m_rc = 0, .m_cs_sz = sizeof(lean_ctor_object) + sizeof(void*)*2 + 0, .m_other = 2, .m_tag = 3}, .m_objs = {((lean_object*)&lp_lean__examples_00_u03b1___closed__1_value),((lean_object*)&lp_lean__examples_q___closed__0_value)}};
+static const lean_object* lp_lean__examples_00_u03c8___closed__0 = (const lean_object*)&lp_lean__examples_00_u03c8___closed__0_value;
+static const lean_ctor_object lp_lean__examples_00_u03c8___closed__1_value = {.m_header = {.m_rc = 0, .m_cs_sz = sizeof(lean_ctor_object) + sizeof(void*)*2 + 0, .m_other = 2, .m_tag = 3}, .m_objs = {((lean_object*)&lp_lean__examples_00_u03b2___closed__0_value),((lean_object*)&lp_lean__examples_p___closed__0_value)}};
+static const lean_object* lp_lean__examples_00_u03c8___closed__1 = (const lean_object*)&lp_lean__examples_00_u03c8___closed__1_value;
+static lean_once_cell_t lp_lean__examples_00_u03c8___closed__2_once = LEAN_ONCE_CELL_INITIALIZER;
+static lean_object* lp_lean__examples_00_u03c8___closed__2;
+LEAN_EXPORT lean_object* lp_lean__examples_00_u03c8;
+LEAN_EXPORT lean_object* _lean_main(){
 _start:
 {
-lean_object* x_3; lean_object* x_4; lean_object* x_5; 
-x_3 = lean_get_stdout();
-x_4 = lean_ctor_get(x_3, 4);
-lean_inc_ref(x_4);
-lean_dec_ref(x_3);
-x_5 = lean_apply_2(x_4, x_1, lean_box(0));
-return x_5;
+lean_object* v___x_2_; lean_object* v___x_3_; 
+v___x_2_ = lean_box(0);
+v___x_3_ = lean_alloc_ctor(0, 1, 0);
+lean_ctor_set(v___x_3_, 0, v___x_2_);
+return v___x_3_;
 }
 }
-LEAN_EXPORT lean_object* lp_lean__examples_IO_print___at___00IO_println___at___00main_spec__0_spec__0___boxed(lean_object* x_1, lean_object* x_2) {
+LEAN_EXPORT lean_object* lp_lean__examples_main___boxed(lean_object* v_a_4_){
 _start:
 {
-lean_object* x_3; 
-x_3 = lp_lean__examples_IO_print___at___00IO_println___at___00main_spec__0_spec__0(x_1);
-return x_3;
+lean_object* v_res_5_; 
+v_res_5_ = _lean_main();
+return v_res_5_;
 }
 }
-LEAN_EXPORT lean_object* lp_lean__examples_IO_println___at___00main_spec__0(lean_object* x_1) {
+LEAN_EXPORT uint8_t lp_lean__examples_I(lean_object* v_x_16_){
 _start:
 {
-uint32_t x_3; lean_object* x_4; lean_object* x_5; 
-x_3 = 10;
-x_4 = lean_string_push(x_1, x_3);
-x_5 = lp_lean__examples_IO_print___at___00IO_println___at___00main_spec__0_spec__0(x_4);
-return x_5;
+lean_object* v___x_17_; uint8_t v___x_18_; 
+v___x_17_ = ((lean_object*)(lp_lean__examples_f___closed__0));
+v___x_18_ = lean_string_dec_eq(v_x_16_, v___x_17_);
+if (v___x_18_ == 0)
+{
+lean_object* v___x_19_; uint8_t v___x_20_; 
+v___x_19_ = ((lean_object*)(lp_lean__examples_f___closed__2));
+v___x_20_ = lean_string_dec_eq(v_x_16_, v___x_19_);
+return v___x_20_;
+}
+else
+{
+return v___x_18_;
 }
 }
-LEAN_EXPORT lean_object* lp_lean__examples_IO_println___at___00main_spec__0___boxed(lean_object* x_1, lean_object* x_2) {
+}
+LEAN_EXPORT lean_object* lp_lean__examples_I___boxed(lean_object* v_x_21_){
 _start:
 {
-lean_object* x_3; 
-x_3 = lp_lean__examples_IO_println___at___00main_spec__0(x_1);
-return x_3;
+uint8_t v_res_22_; lean_object* v_r_23_; 
+v_res_22_ = lp_lean__examples_I(v_x_21_);
+lean_dec_ref(v_x_21_);
+v_r_23_ = lean_box(v_res_22_);
+return v_r_23_;
 }
 }
-static lean_object* _init_lp_lean__examples_main___closed__0() {
+static lean_object* _init_lp_lean__examples_model(void){
 _start:
 {
-lean_object* x_1; 
-x_1 = lean_mk_string_unchecked("Hello, world!", 13, 13);
-return x_1;
+lean_object* v___x_24_; 
+v___x_24_ = lean_box(0);
+return v___x_24_;
 }
 }
-LEAN_EXPORT lean_object* _lean_main() {
+static lean_object* _init_lp_lean__examples_00_u03c8___closed__2(void){
 _start:
 {
-lean_object* x_2; lean_object* x_3; 
-x_2 = lp_lean__examples_main___closed__0;
-x_3 = lp_lean__examples_IO_println___at___00main_spec__0(x_2);
-return x_3;
+lean_object* v___x_53_; lean_object* v___x_54_; lean_object* v___x_55_; 
+v___x_53_ = ((lean_object*)(lp_lean__examples_00_u03c8___closed__1));
+v___x_54_ = ((lean_object*)(lp_lean__examples_00_u03c8___closed__0));
+v___x_55_ = lp_lean__examples_Logic_DL_conj(v___x_54_, v___x_53_);
+return v___x_55_;
 }
 }
-LEAN_EXPORT lean_object* lp_lean__examples_main___boxed(lean_object* x_1) {
+static lean_object* _init_lp_lean__examples_00_u03c8(void){
 _start:
 {
-lean_object* x_2; 
-x_2 = _lean_main();
-return x_2;
+lean_object* v___x_56_; 
+v___x_56_ = lean_obj_once(&lp_lean__examples_00_u03c8___closed__2, &lp_lean__examples_00_u03c8___closed__2_once, _init_lp_lean__examples_00_u03c8___closed__2);
+return v___x_56_;
 }
 }
 lean_object* initialize_Init(uint8_t builtin);
-lean_object* initialize_lean__examples_LeanExamples(uint8_t builtin);
+lean_object* initialize_lean__examples_Logic_Prop_Syntax(uint8_t builtin);
+lean_object* initialize_lean__examples_Logic_Prop_Semantics(uint8_t builtin);
+lean_object* initialize_lean__examples_Logic_DL_Syntax(uint8_t builtin);
+lean_object* initialize_lean__examples_Logic_DL_Semantics(uint8_t builtin);
 static bool _G_initialized = false;
 LEAN_EXPORT lean_object* initialize_lean__examples_Main(uint8_t builtin) {
 lean_object * res;
@@ -95,47 +143,57 @@ _G_initialized = true;
 res = initialize_Init(builtin);
 if (lean_io_result_is_error(res)) return res;
 lean_dec_ref(res);
-res = initialize_lean__examples_LeanExamples(builtin);
+res = initialize_lean__examples_Logic_Prop_Syntax(builtin);
 if (lean_io_result_is_error(res)) return res;
 lean_dec_ref(res);
-lp_lean__examples_main___closed__0 = _init_lp_lean__examples_main___closed__0();
-lean_mark_persistent(lp_lean__examples_main___closed__0);
+res = initialize_lean__examples_Logic_Prop_Semantics(builtin);
+if (lean_io_result_is_error(res)) return res;
+lean_dec_ref(res);
+res = initialize_lean__examples_Logic_DL_Syntax(builtin);
+if (lean_io_result_is_error(res)) return res;
+lean_dec_ref(res);
+res = initialize_lean__examples_Logic_DL_Semantics(builtin);
+if (lean_io_result_is_error(res)) return res;
+lean_dec_ref(res);
+lp_lean__examples_model = _init_lp_lean__examples_model();
+lean_mark_persistent(lp_lean__examples_model);
+lp_lean__examples_00_u03c8 = _init_lp_lean__examples_00_u03c8();
+lean_mark_persistent(lp_lean__examples_00_u03c8);
 return lean_io_result_mk_ok(lean_box(0));
 }
 char ** lean_setup_args(int argc, char ** argv);
 void lean_initialize_runtime_module();
-
-  #if defined(WIN32) || defined(_WIN32)
-  #include <windows.h>
-  #endif
-
-  int main(int argc, char ** argv) {
-  #if defined(WIN32) || defined(_WIN32)
+#if defined(WIN32) || defined(_WIN32)
+#include <windows.h>
+#endif
+lean_object* run_main(int argc, char ** argv) {
+    return _lean_main();
+}
+int main(int argc, char ** argv) {
+#if defined(WIN32) || defined(_WIN32)
   SetErrorMode(SEM_FAILCRITICALERRORS);
   SetConsoleOutputCP(CP_UTF8);
-  #endif
-  lean_object* in; lean_object* res;
-argv = lean_setup_args(argc, argv);
-lean_initialize_runtime_module();
-lean_set_panic_messages(false);
-res = initialize_lean__examples_Main(1 /* builtin */);
-lean_set_panic_messages(true);
-lean_io_mark_end_initialization();
-if (lean_io_result_is_ok(res)) {
-lean_dec_ref(res);
-lean_init_task_manager();
-res = _lean_main();
-}
-lean_finalize_task_manager();
-if (lean_io_result_is_ok(res)) {
-  int ret = 0;
-  lean_dec_ref(res);
-  return ret;
-} else {
-  lean_io_result_show_error(res);
-  lean_dec_ref(res);
-  return 1;
-}
+#endif
+  lean_object* res;
+  argv = lean_setup_args(argc, argv);
+  lean_initialize_runtime_module();
+  res = initialize_lean__examples_Main(1 /* builtin */);
+  lean_io_mark_end_initialization();
+  if (lean_io_result_is_ok(res)) {
+    lean_dec_ref(res);
+    lean_init_task_manager();
+    res = lean_run_main(&run_main, argc, argv);
+  }
+  lean_finalize_task_manager();
+  if (lean_io_result_is_ok(res)) {
+    int ret = 0;
+    lean_dec_ref(res);
+    return ret;
+  } else {
+    lean_io_result_show_error(res);
+    lean_dec_ref(res);
+    return 1;
+  }
 }
 #ifdef __cplusplus
 }
