Logic/DL/Proofs.lean
@@ -1,0 +1,46 @@
+import Logic.DL.Semantics
+
+namespace Logic.DL
+
+open DLForm
+open Relation
+set_option trace.Meta.Tactic.simp.rewrite true
+
+--formulas are equivalent to themselves
+theorem equiv_refl (φ: DLForm):
+  equiv φ φ :=
+  by
+    simp[equiv]
+
+--and evaluates correct wrt to ∧
+theorem and_correct (φ ψ: DLForm):
+  ∀ M s, eval M (conj φ ψ) s ↔ (eval M φ s) ∧ (eval M ψ s) :=
+  by
+    intro M s
+    simp[conj, not, eval]
+-- anything follows from ⊥
+theorem ex_falso (φ: DLForm):
+  eval M falsum n → eval M φ n :=
+  by
+    intro h
+    simp[eval] at h
+
+
+-- transition s -> s' with some a implies transition s -> s' with wildcard
+theorem ato_imp_wild (M: KripkeModel) (a s s': Nat) :
+  evalRel M (Relation.relAtom a) s s' → evalRel M Relation.wild s s' :=
+  by
+  intro h
+  simp[evalRel] at h
+  simp[evalRel]
+  exact ⟨a, h⟩
+
+-- transition s -> s' with wildcard implies there exist atomic rel with s -> s'
+theorem wild_imp_ato (M: KripkeModel):
+  evalRel M Relation.wild s s' → ∃a, evalRel M (Relation.relAtom a) s s' :=
+  by
+  intro h
+  simp[evalRel] at *
+  exact h
+
+end Logic.DL
