Logic/DL/Syntax.lean
@@ -1,0 +1,37 @@
+import Logic.Prop.Syntax
+
+namespace Logic.DL
+
+inductive Relation : Type
+  | relAtom : Nat → Relation -- atomic relations modelled as natural numbers
+  | anywhere : Relation --
+  | wild : Relation -- wildcard •
+  | comp : Relation → Relation → Relation -- composition α.β
+  | alt : Relation → Relation → Relation -- alternation α ∪ β
+  | iter : Relation → Relation --iteration α*
+
+inductive DLForm : Type
+  | atom : String → DLForm -- atomic propositions modelled as strings
+  | falsum : DLForm -- falsum ⊥
+  | imp : DLForm → DLForm → DLForm -- implication φ → ψ
+  | diamond : Relation → DLForm → DLForm -- diamond ⟨α⟩φ
+
+--derived syntactic sugar
+open DLForm
+
+-- negation ¬φ
+def not (φ : DLForm) : DLForm := imp φ falsum
+
+-- true ⊤
+def true : DLForm := not falsum
+
+--conjunction φ ∧ ψ
+def conj (φ ψ: DLForm) : DLForm := not (imp φ (not ψ))
+
+--disjunction φ ∨ ψ
+def disj (φ ψ: DLForm) : DLForm := imp (not φ) ψ
+
+--box [α]φ
+def box (α: Relation) (φ: DLForm) : DLForm := not (diamond α (not φ))
+
+end Logic.DL
