Logic/Prop/Nnf.lean
@@ -1,0 +1,16 @@
+import Logic.Prop.Semantics
+namespace Logic.Prop
+
+open PropositionalForm
+-- negative normal form
+def nnf : PropositionalForm -> PropositionalForm
+  | var x => var x
+  | myFalse => myFalse
+  | myAnd φ ψ => myAnd (nnf φ) (nnf ψ)
+  | myNot φ => match φ with
+    | var x => myNot (var x)
+    | myFalse => myTrue
+    | myAnd ψ₁ ψ₂ => myOr (nnf (myNot ψ₁)) (nnf (myNot ψ₂))
+    | myNot ψ => nnf ψ
+
+end Logic.Prop
