Logic/Prop/Proofs.lean
@@ -1,0 +1,92 @@
+import Logic.Prop.Nnf
+
+namespace Logic.Prop
+
+open PropositionalForm
+set_option trace.Meta.Tactic.simp.rewrite true --show verbose infoview
+
+
+--some simple proofs
+
+-- prove deMorgans law
+theorem DeMorgan (φ ψ: PropositionalForm):
+  equiv (myNot (myAnd φ ψ))  (myOr (myNot φ) (myNot ψ)) :=
+  by
+    intro v --"take an arbitrary valuation v"
+    simp[eval, myOr] --"simplify by using definitions of eval, myOr"
+
+
+-- prove ¬¬φ ≃ φ
+theorem DoubleNeg (φ: PropositionalForm):
+  equiv (myNot (myNot φ)) φ :=
+  by
+    intro v
+    calc
+      eval v (myNot (myNot φ))
+        = ! (eval v (myNot φ)) := by rfl
+      _ = !(!(eval v  φ)) := by rfl
+      _ = eval v φ := by rewrite[Bool.not_not]; rfl
+
+
+--prove φ → ψ ≃ ¬φ ∨ ψ
+theorem Imp (φ ψ: PropositionalForm):
+  equiv (imp φ ψ)  (myOr (myNot φ) ψ) :=
+  by
+    intro v
+    rfl
+
+
+--prove φ ∧ ψ ≃ ψ ∧ φ
+theorem AndComm (φ ψ: PropositionalForm):
+  equiv (myAnd φ ψ) (myAnd ψ φ) :=
+  by
+    intro v
+    simp[eval, Bool.and_comm]
+
+--a little more verbose
+theorem AndComm' (φ ψ: PropositionalForm):
+  equiv (myAnd φ ψ) (myAnd ψ φ) :=
+  by
+    intro v
+    unfold eval
+    rw[Bool.and_comm]
+
+--prove φ ≃ ψ => ¬φ ≃ ψ
+theorem NotCongr (φ ψ: PropositionalForm):
+  equiv φ ψ -> equiv (myNot φ) (myNot ψ) :=
+  by
+    intro h v
+    simp[eval, h v]
+
+--prove equivalence is transitive
+theorem EquivTrans (φ ψ ρ: PropositionalForm):
+  equiv φ ψ -> equiv ψ ρ -> equiv φ ρ :=
+  by
+    intro h₁ h₂ v
+    simp[h₁ v, h₂ v]
+
+
+
+--prove that the nnf of φ is equivalent to φ
+theorem NNFEquiv (φ: PropositionalForm):
+  equiv (nnf φ) φ ∧ equiv (nnf (myNot φ)) (myNot φ) := --including the negated version to obtain a suitable hypothesis ih.2 for myNot case
+  by
+    induction φ with
+    | var x =>
+      constructor -- apply And.intro (constructor) to split conjunction target
+      case left => intro v; rw[nnf] -- equiv (nnf φ) φ
+      case right => intro v; rw[nnf] -- equiv (nnf (myNot φ)) (myNot φ)
+    | myFalse =>
+      constructor
+      case left => intro v; rw[nnf]
+      case right => intro v; simp[nnf, eval, myTrue]
+    | myAnd ψ₁ ψ₂ ih₁ ih₂ => --e.g. ih₁ is induction hypothesis for ψ₁
+      constructor
+      case left => intro v; simp[nnf, eval, ih₁.1 v, ih₂.1 v]
+      case right => intro v; simp[nnf, eval, ih₁.2 v, ih₂.2 v, myOr] --nnf of negation  transformed into myOr
+    | myNot ψ ih =>
+      constructor
+      case left => exact ih.2 --equiv
+      case right => intro v; simp[nnf, eval, ih.1 v]
+
+end Logic.Prop
