Logic/Prop/Semantics.lean
@@ -1,0 +1,17 @@
+import Logic.Prop.Syntax
+
+namespace Logic.Prop
+-- propositional evaluation
+def Valuation := String -> Bool
+
+def eval (v : Valuation) : PropositionalForm -> Bool
+  | PropositionalForm.var x => v x
+  | PropositionalForm.myFalse => false
+  | PropositionalForm.myAnd φ ψ => eval v φ && eval v ψ
+  | PropositionalForm.myNot φ => ! eval v φ
+
+-- logic equivalence
+def equiv (φ ψ: PropositionalForm) : Prop :=
+  ∀ v, eval v φ = eval v ψ
+
+end Logic.Prop
