Logic/Prop/Syntax.lean
@@ -1,0 +1,19 @@
+
+namespace Logic.Prop
+
+-- Representation of propositional formulas
+inductive PropositionalForm : Type
+  | var : String -> PropositionalForm
+  | myFalse : PropositionalForm
+  | myNot : PropositionalForm -> PropositionalForm
+  | myAnd : PropositionalForm -> PropositionalForm -> PropositionalForm
+
+-- Syntactic sugar for additional connectives
+def myOr (p q: PropositionalForm): PropositionalForm :=
+  PropositionalForm.myNot (PropositionalForm.myAnd (PropositionalForm.myNot p) (PropositionalForm.myNot q))
+
+def myTrue : PropositionalForm := PropositionalForm.myNot PropositionalForm.myFalse
+
+def imp (p q: PropositionalForm): PropositionalForm := myOr (PropositionalForm.myNot p) q
+
+end Logic.Prop
